Vcg_Quadruple.v
@@ -5,9 +5,10 @@ From Rela Require Import Sem.
 From Rela Require Import Sigma.
 From Rela Require Import Hoare_Triple.
 From Rela Require Import Quadruple.
+From Rela Require Import Vcg.
 From Rela Require Import Vcg_Rela.
 
-From Coq Require Import Lists.List.
+From Stdlib Require Import Lists.List.
 Import ListNotations.
 
 (** Defintion of the verification condition generator for quadruples,
@@ -15,47 +16,47 @@ Import ListNotations.
 
 Definition q_suite : Type := Sigma.sigma -> Sigma.sigma -> history ->  history -> Prop.
 
-Definition to_rsuite (suite: q_suite) : r_suite :=
-  fun ml hl => match ml, hl with
-            | m1 :: m2 :: [], h1 :: h2 :: [] => suite m1 m2 h1 h2
-            | _, _ => False
-            end.
-
-Definition qtc (c1 c2: com) (m1 m2: Sigma.sigma) (h1 h2: history)
-  (cls: Phi.phi) (suite: q_suite) : Prop :=
-  let cl := c1 :: [c2] in
-  let ml := m1 :: [m2] in
-  let hl := h1 :: [h2] in
-  rtc cl ml hl cls (to_rsuite suite) eq_refl eq_refl.
+Definition qtc
+  (c1 c2: com)
+  (m1 m2: Sigma.sigma)
+  (h1 h2: history)
+  (cl1 cl2: Phi.phi)
+  (suite: q_suite) : Prop :=
+  tc c1 m1 h1 cl1 (fun m1' h1' =>
+                     tc c2 m2 h2 cl2 (fun m2' h2' => suite m1' m2' h1' h2')).
 
 (** Defintion of the generator of auxiliare goals for relational quadruples **)
 
-Definition qtc' (c1 c2: com) (m1 m2: Sigma.sigma) (h1 h2: history)
-  (cls: Phi.phi): Prop :=
-  let cl := c1 :: [c2] in
-  let ml := m1 :: [m2] in
-  let hl := h1 :: [h2] in
-  rtc' cl ml hl cls eq_refl eq_refl.
+Definition qtc'
+  (c1 c2: com)
+  (m1 m2: Sigma.sigma)
+  (h1 h2: history)
+  (cl1 cl2: Phi.phi): Prop :=
+  tc' c1 m1 h1 cl1 /\ tc' c2 m2 h2 cl2.
 
 (** Defintion of the verification condition generator for quadruple on loop **)
 
-Definition qwtc (c1 c2 : com) (h1 h2: history)
-  (cls: Phi.phi) (inv : q_assertion) (L R : q_cond) b1 b2: Prop :=
+Definition qwtc
+  (c1 c2 : com)
+  (h1 h2: history)
+  (cl: Phi.phi)
+  (inv : q_assertion)
+  (L R : q_cond) b1 b2: Prop :=
   (forall m1 m2,
       inv m1 m2 -> Assn_b.bassn b1 m1 -> Assn_b.bassn b2 m2 ->
       L m1 m2 = false -> R m1 m2 = false ->
-      (qtc' c1 c2 m1 m2 h1 h2 cls /\
-         qtc c1 c2 m1 m2 h1 h2 cls (fun m1' m2' _ _ =>  inv m1' m2')))
+      (qtc' c1 c2 m1 m2 h1 h2 cl cl /\
+         qtc c1 c2 m1 m2 h1 h2 cl cl (fun m1' m2' _ _ =>  inv m1' m2')))
   /\
     (forall m1 m2,
         inv m1 m2 -> Assn_b.bassn b1 m1 -> L m1 m2 = true  ->
-        (qtc' c1 CSkip m1 m2 h1 h2 cls /\
-           qtc c1 CSkip m1 m2 h1 h2 cls (fun m1' m2' _ _ =>  inv m1' m2')))
+        (qtc' c1 CSkip m1 m2 h1 h2 cl cl /\
+           qtc c1 CSkip m1 m2 h1 h2 cl cl (fun m1' m2' _ _ =>  inv m1' m2')))
   /\
     (forall m1 m2,
         inv m1 m2-> Assn_b.bassn b2 m2 -> R m1 m2 = true ->
-        (qtc' CSkip c2 m1 m2 h1 h2 cls /\
-           qtc CSkip c2 m1 m2 h1 h2 cls (fun m1' m2' _ _ =>  inv m1' m2')))
+        (qtc' CSkip c2 m1 m2 h1 h2 cl cl /\
+           qtc CSkip c2 m1 m2 h1 h2 cl cl (fun m1' m2' _ _ =>  inv m1' m2')))
   /\
     (forall m1 m2, inv m1 m2 ->
               beval m1 b1 = beval m2 b2 \/
@@ -67,15 +68,15 @@ Definition qwtc (c1 c2 : com) (h1 h2: history)
 Definition while_call b p inv var ps s s' id :=
   ceval (CWhile b p inv var id) s ps s'.
 
-Definition twq (qwl: QW_Phi.phi) ps :=
+Definition twq (qwl: QW_Phi.phi) ps1 ps2 :=
   forall c1 c2 b1 b2 inv1 inv2 var1 var2 s1 s1' s2 s2' n1 n2,
-    while_call b1 c1 inv1 var1 ps s1 s1' n1 ->
-    while_call b2 c2 inv2 var2 ps s2 s2' n2 ->
+    while_call b1 c1 inv1 var1 ps1 s1 s1' n1 ->
+    while_call b2 c2 inv2 var2 ps2 s2 s2' n2 ->
     get_wq_inv (qwl c1 b1 n1 c2 b2 n2 ) s1 s2 ->
     get_wq_inv (qwl c1 b1 n1 c2 b2 n2 ) s1' s2' /\
       beval s1' b1 = false /\ beval s2' b2 = false.
 
-Lemma tr_quadruple_while (qwl: QW_Phi.phi) ps :
+Lemma tr_quadruple_while (qwl: QW_Phi.phi) ps1 ps2 :
   (forall inv1 inv2 var1 var2 c1 c2 b1 b2 id1 id2,
       let wq_clause := qwl c1 b1 id1 c2 b2 id2 in
       let q_inv := get_wq_inv wq_clause in
@@ -83,8 +84,8 @@ Lemma tr_quadruple_while (qwl: QW_Phi.phi) ps :
         (fun m1 m2  _ _ => q_inv m1 m2 /\
                           beval m1 b1 = false /\ beval m2 b2 = false)
         (CWhile b1 c1 inv1 var1 id1)
-        (CWhile b2 c2 inv2 var2 id2) ps)
-  -> twq qwl ps.
+        (CWhile b2 c2 inv2 var2 id2) ps1 ps2)
+  -> twq qwl ps1 ps2.
 Proof.
 intros H c1 c2 b1 b2 inv1 inv2 var1 var2 s1 s1' s2 s2' id1 id2 hw1 hw2 hinv.
 eapply H;eauto.
@@ -135,73 +136,72 @@ Proof.
       + eapply E_WhileTrue;[assumption | apply IHc;eauto|auto].
 Qed.
 
-(* Lemma inv_call_hoare : *)
-(*   forall (inv: assertion) (var: variant) b c ps l id si, *)
-(*     hoare_triple (fun s => inv (s :: (si :: l))) *)
-(*       (fun s' _ => inv (s' :: (si :: l)) /\ beval s'  b = false) *)
-(*       (CWhile b c inv var id) ps -> *)
-(*     hoare_triple (fun s => inv (s :: (si :: l))) *)
-(*       (fun s' _ => inv (s' :: (si :: l)) /\ beval s'  b = false) *)
-(*       (inv_call (CWhile b c inv var id) ps) ps. *)
-(* Proof. *)
-(*   intros. *)
-(*   intros s s' HPre Heval. *)
-(*   eapply H;[apply HPre | apply inv_call_ceval;auto]. *)
-(* Qed. *)
+Lemma inv_call_hoare :
+  forall (inv: assertion) (var: variant) b c ps l id si,
+    hoare_triple (fun s => inv (s :: (si :: l)))
+      (fun s' _ => inv (s' :: (si :: l)) /\ beval s'  b = false)
+      (CWhile b c inv var id) ps ->
+    hoare_triple (fun s => inv (s :: (si :: l)))
+      (fun s' _ => inv (s' :: (si :: l)) /\ beval s'  b = false)
+      (inv_call (CWhile b c inv var id) ps) ps.
+Proof.
+  intros.
+  intros s s' HPre Heval.
+  eapply H;[apply HPre | apply inv_call_ceval;auto].
+Qed.
 
 (** Definition of a verification condition generator for quadruple on procedures **)
 
-Definition qtr (qcl: Q_Phi.phi) (ps: Psi.psi) :=
+Definition qtr (qcl: Q_Phi.phi) (ps1 ps2: Psi.psi) :=
   forall p1 p2 s1 s2 s1' s2',
-    proc_to_pred (p1 :: [p2]) (s1 :: [s2]) (s1' :: [s2']) ps eq_refl eq_refl ->
+    proc_call p1 s1 s1' ps1 /\ proc_call p2 s2 s2' ps2 ->
     (get_q_pre (qcl p1 p2)) s1 s2 -> (get_q_post (qcl p1 p2)) s1' s2' s1 s2.
 
 (** Facts about tr **)
 
-Lemma qtr_relational_prop (qcl:Q_Phi.phi) (ps: Psi.psi):
+Lemma qtr_relational_prop (qcl:Q_Phi.phi) (ps1 ps2: Psi.psi):
   (forall p1 p2,
       quadruple
         (get_q_pre (qcl p1 p2))
         (get_q_post (qcl p1 p2))
-        (CCall p1)  (CCall p2)ps)
-  -> qtr qcl ps.
+        (CCall p1) (CCall p2) ps1 ps2)
+  -> qtr qcl ps1 ps2.
 Proof.
-  intros H  p1 p2 s1 s2 s1' s2' Hcall Hp.
-  apply rceval_proc_to_prod in Hcall.
-  inversion Hcall;subst.
-  inversion H8;subst.
+  intros H p1 p2 s1 s2 s1' s2' [Hcall1 Hcall2] Hp.
   apply H;auto.
 Qed.
 
 (** Definition of a verification condition generator for quadruple on procedures **)
 
-Definition qtc_p (ps: Psi.psi) (cls: Phi.phi) (qcl: Q_Phi.phi): Prop :=
-  forall f1 f2 ps',
-    let c1 := ps f1 in
-    let c2 := ps f2 in
+Definition qtc_p (ps1 ps2: Psi.psi) (qcl: Q_Phi.phi): Prop :=
+  forall f1 f2 ps1' ps2',
+    let c1 := ps1 f1 in
+    let c2 := ps2 f2 in
+    let cl1 := (phi_call Phi.empty_phi ps1') in
+    let cl2 := (phi_call Phi.empty_phi ps2') in
     (forall m1 m2,
         get_q_pre (qcl f1 f2) m1 m2 /\
-          qtr qcl ps' /\
+          qtr qcl ps1' ps2' /\
           get_LR(qcl f1 f2) m1 m2 = true /\
           get_L(qcl f1 f2) m1 m2 = false /\
           get_R(qcl f1 f2) m1 m2 = false ->
-        (qtc' c1 c2 m1 m2 empty_history empty_history (phi_call cls ps') /\
-           qtc c1 c2  m1 m2 empty_history empty_history (phi_call cls ps')
+        (qtc' c1 c2 m1 m2 empty_history empty_history cl1 cl2 /\
+           qtc c1 c2  m1 m2 empty_history empty_history cl1 cl2
              (fun m1' m2' _ _ => (get_q_post (qcl f1 f2)) m1' m2' m1 m2)))
     /\
     (forall m1 m2,
         get_q_pre (qcl f1 f2) m1 m2 /\
-          qtr qcl ps' /\
+          qtr qcl ps1' ps2' /\
           get_L(qcl f1 f2) m1 m2 = true ->
-        (qtc' c1 CSkip m1 m2 empty_history empty_history (phi_call cls ps') /\
-           qtc c1 CSkip  m1 m2 empty_history empty_history (phi_call cls ps')
+        (qtc' c1 (CCall f2) m1 m2 empty_history empty_history cl1 cl2 /\
+           qtc c1 (CCall f2)  m1 m2 empty_history empty_history cl1 cl2
              (fun m1' m2' _ _ => (get_q_post (qcl f1 f2)) m1' m2' m1 m2))) /\
     (forall m1 m2,
         get_q_pre (qcl f1 f2) m1 m2 /\
-          qtr qcl ps' /\
+          qtr qcl ps1' ps2' /\
           get_R(qcl f1 f2) m1 m2 = true ->
-        (qtc' CSkip c2 m1 m2 empty_history empty_history (phi_call cls ps') /\
-           qtc CSkip c2 m1 m2 empty_history empty_history (phi_call cls ps')
+        (qtc' (CCall f1) c2 m1 m2 empty_history empty_history cl1 cl2 /\
+           qtc (CCall f1) c2 m1 m2 empty_history empty_history cl1 cl2
              (fun m1' m2' _ _ => (get_q_post (qcl f1 f2)) m1' m2' m1 m2)))
       /\
         (forall m1 m2,  get_q_pre (qcl f1 f2) m1 m2 ->
