Vcg_Rela.v
@@ -5,8 +5,7 @@ From Rela Require Import Sigma.
 From Rela Require Import Hoare_Triple.
 From Rela Require Import Rela.
 
-From Coq Require Import Program.
-From Coq Require Import Lists.List.
+From Stdlib Require Import Lists.List.
 Import ListNotations.
 
 (** Definition of the verification condition generator for relational properties,
@@ -14,100 +13,27 @@ Import ListNotations.
 
 Definition r_suite : Type := list Sigma.sigma -> list history -> Prop.
 
-Program Fixpoint rtc (cl : list com) (ml: list Sigma.sigma) (hl: list history)
-            (cls: Phi.phi) (suite : r_suite)
-            (hy1:length cl = length ml) (hy2:length cl = length hl): Prop :=
- match cl,ml,hl with
- | [],[],[] => suite [] []
- | c :: qc, m :: qm, h :: qh =>
-   tc c m h cls (fun m' h' => rtc qc qm qh cls (fun lm lh => suite (m'::lm) (h' :: lh)) _ _)
- | _,_,_ => !
+Fixpoint rtc
+  (cl : list com) (ml: list Sigma.sigma) (hl: list history)
+  (cls: Phi.phi) (suite : r_suite): Prop :=
+  match cl,ml,hl with
+  | [],[],[] => suite [] []
+  | c :: qc, m :: qm, h :: qh =>
+      tc c m h cls (fun m' h' => rtc qc qm qh cls (fun lm lh => suite (m'::lm) (h' :: lh)))
+ | _,_,_ => False
 end.
-
-Next Obligation.
-destruct cl.
-- simpl in hy1.
-  symmetry in hy1.
-  apply length_zero_iff_nil in hy1.
-  simpl in hy2.
-  symmetry in hy2.
-  apply length_zero_iff_nil in hy2.
-  subst ml hl.
-  contradiction H0.
-  split.
-  reflexivity.
-  split.
-  reflexivity. reflexivity.
-- destruct ml as [|m qm].
-  discriminate hy1.
-  destruct hl as [|h hm].
-  discriminate hy2.
-  eapply H.
-  split.
-  reflexivity.
-  split.
-  reflexivity. reflexivity.
-Qed.
-
-Next Obligation.
-split.
-intros.
-intros contra.
-destruct contra as (contra & _).
-discriminate contra.
-intros contra.
-destruct contra as ( _ & contra).
-destruct contra as ( _ & contra).
-discriminate contra.
-Defined.
-
-Next Obligation.
-split.
-intros.
-intros contra.
-destruct contra as ( _ & contra).
-destruct contra as (contra & _).
-discriminate contra.
-intros contra.
-destruct contra as (contra & _).
-discriminate contra.
-Defined.
-
-Next Obligation.
-split.
-intros.
-intros contra.
-destruct contra as (contra & _).
-discriminate contra.
-intros contra.
-destruct contra as (_ & contra ).
-destruct contra as (contra & _).
-discriminate contra.
-Defined.
-
-Next Obligation.
-split.
-intros.
-intros contra.
-destruct contra as (_ & contra ).
-destruct contra as (_ & contra ).
-discriminate contra.
-intros contra.
-destruct contra as (contra & _).
-discriminate contra.
-Defined.
 
 (** Connect between Hoare Triple and Relational Properties **)
 
 Lemma hoare_rela :
-forall (P: r_precondition) (Q: r_postcondition)
-h q ps pi sl hl (hy1:length q = length sl) (hy2:length q = length hl),
-(forall s2 s3 : sigma,
-P (s2 :: sl) -> ceval h s2 ps s3 ->
-rtc q sl hl pi (fun sl' _ => Q (s3 :: sl') (s2 :: sl)) hy1 hy2) =
-hoare_triple (fun s => P (s:: sl) )
-     (fun s' s => rtc q sl hl pi (fun sl' _ => Q (s' :: sl') (s :: sl)) hy1 hy2)
-              h ps.
+  forall (P: r_precondition) (Q: r_postcondition)
+    h q ps cll sl hl,
+    (forall s2 s3 : sigma,
+        P (s2 :: sl) -> ceval h s2 ps s3 ->
+        rtc q sl hl cll (fun sl' _ => Q (s3 :: sl') (s2 :: sl))) =
+      hoare_triple (fun s => P (s:: sl) )
+        (fun s' s => rtc q sl hl cll (fun sl' _ => Q (s' :: sl') (s :: sl)))
+        h ps.
 Proof.
 intros.
 unfold hoare_triple.
@@ -116,254 +42,55 @@ Qed.
 
 (** Defintion of the generator of auxiliare goals for relational properties **)
 
-Program Fixpoint rtc' (cl : list com) (ml: list Sigma.sigma)
-            (hl: list history) (cls : Phi.phi)
-            (hy1:length cl = length ml) (hy2:length cl = length hl): Prop :=
- match cl,ml,hl with
- | [],[],[] => True
- | c :: qc, m :: qm, h :: qh =>
-   tc' c m h cls /\ rtc' qc qm qh cls _ _
- | _,_, _ => !
-end.
-
-Next Obligation.
-destruct cl.
-- simpl in hy1.
-  symmetry in hy1.
-  apply length_zero_iff_nil in hy1.
-  simpl in hy2.
-  symmetry in hy2.
-  apply length_zero_iff_nil in hy2.
-  subst ml.
-  subst hl.
-  contradiction H0.
-  split.
-  reflexivity.
-  split.
-  reflexivity. reflexivity.
-- destruct ml as [|m qm].
-  discriminate hy1.
-  destruct hl as [|h qh].
-  discriminate hy2.
-  eapply H.
-  split.
-  reflexivity.
-  split.
-  reflexivity. reflexivity.
-Qed.
-
-Next Obligation.
-split.
-intros.
-intros contra.
-destruct contra as (contra & _).
-discriminate contra.
-intros contra.
-destruct contra as ( _ & contra).
-destruct contra as ( _ & contra).
-discriminate contra.
-Defined.
-
-Next Obligation.
-split.
-intros.
-intros contra.
-destruct contra as ( _ & contra).
-destruct contra as (contra & _).
-discriminate contra.
-intros contra.
-destruct contra as (contra & _).
-discriminate contra.
-Defined.
-
-Next Obligation.
-split.
-intros.
-intros contra.
-destruct contra as (contra & _).
-discriminate contra.
-intros contra.
-destruct contra as (_ & contra ).
-destruct contra as (contra & _).
-discriminate contra.
-Defined.
-
-Next Obligation.
-split.
-intros.
-intros contra.
-destruct contra as (_ & contra ).
-destruct contra as (_ & contra ).
-discriminate contra.
-intros contra.
-destruct contra as (contra & _).
-discriminate contra.
-Defined.
-
-(** Facts about rtc and rtc' **)
-
-Lemma mk_rtc_def :
-forall c q pi s sl h hl
-(hy1:length (c::q) = length (s::sl)) (hy2:length (c::q) = length (h::hl)),
-exists (hyr1:length q = length sl),
-exists (hyr2:length q = length hl),
-forall P,
-rtc (c :: q) (s::sl) (h::hl) pi P hy1 hy2  =
-tc c s h pi (fun m' h' => rtc q sl hl pi (fun ml hl => P (m'::ml) (h'::hl)) hyr1 hyr2).
-Proof.
-intros.
-eexists.
-eexists.
-program_simpl.
-Qed.
-
-Lemma mk_rtc'_def :
-forall c q pi s sl h hl
-(hy1:length (c::q) = length (s::sl))
-(hy2:length (c::q) = length (h::hl)),
-exists (hyr1:length q = length sl),
-exists (hyr2:length q = length hl),
-rtc' (c :: q) (s::sl) (h::hl)pi hy1 hy2  =
-(tc' c s h pi /\ rtc' q sl hl pi hyr1 hyr2).
-Proof.
-intros.
-eexists.
-eexists.
-program_simpl.
-Qed.
+Fixpoint rtc'
+  (cl : list com)
+  (ml: list Sigma.sigma)
+  (hl: list history)
+  (cls : Phi.phi): Prop :=
+  match cl,ml,hl with
+  | [],[],[] => True
+  | c :: qc, m :: qm, h :: qh =>
+      tc' c m h cls /\ rtc' qc qm qh cls
+  | _,_,_ => False
+  end.
 
 (** Translation of a list of procedure call to Prop **)
 
 Definition proc_call f s s' ps := ceval (CCall f) s ps s'.
 
-Program Fixpoint proc_to_pred p s s' ps (hy1:length p = length s)
-                                        (hy2:length p = length s'): Prop:=
-match p, s, s' with
-| [] , [], [] => True
-| h :: q, s:: qs, s' :: qs' => proc_call h s s' ps /\ proc_to_pred q qs qs' ps _ _
-| _, _, _ => !
-end.
+Fixpoint proc_to_pred p s s' ps : Prop:=
+  match p, s, s' with
+  | [] , [], [] => True
+  | h :: q, s:: qs, s' :: qs' =>
+      proc_call h s s' ps /\ proc_to_pred q qs qs' ps
+  | _, _, _ => False
+  end.
 
-Next Obligation.
-destruct p.
-- simpl in hy1.
-  symmetry in hy1.
-  apply length_zero_iff_nil in hy1.
-  simpl in hy2.
-  symmetry in hy2.
-  apply length_zero_iff_nil in hy2.
-  subst s.
-  subst s'.
-  contradiction H0.
-  split.
-  reflexivity.
-  split.
-  reflexivity. reflexivity.
-- destruct s as [|s qs].
-  discriminate hy1.
-  destruct s' as [|s' qs'].
-  discriminate hy2.
-  eapply H.
-  split.
-  reflexivity.
-  split.
-  reflexivity. reflexivity.
-Qed.
-
-Next Obligation.
-split.
-intros.
-intros contra.
-destruct contra as (contra & _).
-discriminate contra.
-intros contra.
-destruct contra as ( _ & contra).
-destruct contra as ( _ & contra).
-discriminate contra.
-Defined.
-
-Next Obligation.
-split.
-intros.
-intros contra.
-destruct contra as ( _ & contra).
-destruct contra as (contra & _).
-discriminate contra.
-intros contra.
-destruct contra as (contra & _).
-discriminate contra.
-Defined.
-
-Next Obligation.
-split.
-intros.
-intros contra.
-destruct contra as (contra & _).
-discriminate contra.
-intros contra.
-destruct contra as (_ & contra ).
-destruct contra as (contra & _).
-discriminate contra.
-Defined.
-
-Next Obligation.
-split.
-intros.
-intros contra.
-destruct contra as (_ & contra ).
-destruct contra as (_ & contra ).
-discriminate contra.
-intros contra.
-destruct contra as (contra & _).
-discriminate contra.
-Defined.
-
-(** Facts about proc_to_pred **)
-
-Lemma mk_proc_to_pred_def :
-forall c q s sl s' sl' ps
-(hy1:length (c::q) = length (s::sl)) (hy2:length (c::q) = length (s'::sl')),
-exists (hyr1:length q = length sl),
-exists (hyr2:length q = length sl'),
-proc_to_pred (c :: q) (s::sl) (s'::sl') ps hy1 hy2  =
-(proc_call c s s' ps /\ proc_to_pred q sl sl' ps hyr1 hyr2).
+Lemma rceval_proc_to_prod  p s s' ps :
+  proc_to_pred p s s' ps  -> rceval (fold_call p) s ps s' .
 Proof.
-intros.
-eexists.
-eexists.
-program_simpl.
-Qed.
-
-Lemma rceval_proc_to_prod p s s' ps (hy1:length p = length s) (hy2:length p = length s') :
-proc_to_pred p s s' ps hy1 hy2 -> rceval (fold_call p) s ps s' .
-Proof.
-generalize dependent hy2.
-generalize dependent hy1.
 generalize dependent s'.
 generalize dependent s.
+generalize dependent ps.
 induction p; intros.
-  + destruct s;[| discriminate hy1].
-    destruct s';[| discriminate hy2].
-    simpl. apply E_Empty.
-  + destruct s;[discriminate hy1| ].
-    destruct s';[discriminate hy2| ].
-    specialize (mk_proc_to_pred_def a p s s0 s1 s' ps hy1 hy2) as (hyr1 & hyr2 & HYP).
-    rewrite HYP in H.
-    simpl.
-    apply E_Seq.
-    -  apply H.
-    - inversion hy1.
-      inversion hy2.
-     apply IHp with (hy1:= hyr1)(hy2:= hyr2). apply H.
+- destruct s ;[|contradiction H].
+  destruct s';[|contradiction H].
+  apply E_Empty.
+- destruct s ;[contradiction H|].
+  destruct s';[contradiction H|].
+  simpl.
+  apply E_Seq.
+  + apply H.
+  + apply IHp. apply H.
 Qed.
 
 (** Translation of a relational contract into Prop **)
 
 Definition tr (rcl:R_Phi.phi) ps :=
-   forall p s s' (hy1:length p = length s) (hy2:length p = length s'),
-          0 < length p ->
-          proc_to_pred p s s' ps hy1 hy2 ->
-          (get_r_pre (rcl p)) s -> (get_r_post (rcl p)) s' s.
+  forall p s s',
+    0 < length p ->
+    proc_to_pred p s s' ps ->
+    (get_r_pre (rcl p)) s -> (get_r_post (rcl p)) s' s.
 
 (** Facts about tr **)
 
@@ -372,28 +99,51 @@ Lemma tr_relational_prop (rcl:R_Phi.phi) (ps: Psi.psi):
      relational_prop (get_r_pre (rcl p)) (get_r_post (rcl p)) (fold_call p) ps)
           -> tr rcl ps.
 Proof.
-intros H p s s' hy1 hy2 hy Hcall Hrp.
+  intros H p s s' Hp Hcall HPre.
   apply H.
-  + apply hy.
-  + rewrite fold_call_length.
-    symmetry. assumption.
-  + rewrite fold_call_length.
-    symmetry. assumption.
-  + assumption.
-  + eapply rceval_proc_to_prod in Hcall.
+  - assumption.
+  - rewrite fold_call_length.
+    revert Hcall.
+    clear.
+    revert s. revert s'.
+    induction p;intros.
+    + destruct s;[reflexivity| contradiction Hcall].
+    + destruct s;[contradiction Hcall|].
+      simpl. f_equal.
+      destruct s';[contradiction Hcall|].
+      eapply IHp.
+      apply Hcall.
+  - rewrite fold_call_length.
+    revert Hcall.
+    clear.
+    revert s. revert s'.
+    induction p;intros.
+    + destruct s;[|contradiction Hcall].
+      destruct s';[reflexivity|contradiction Hcall].
+    + destruct s;[contradiction Hcall|].
+      destruct s';[contradiction Hcall|].
+      simpl. f_equal.
+      eapply IHp.
+      apply Hcall.
+  - assumption.
+  - eapply rceval_proc_to_prod in Hcall.
     apply Hcall.
 Qed.
 
 (** Adding proc_call to post condition of procedure contract **)
 
 Definition phi_call (cl : Phi.phi) ps :=
-    fun x => (get_pre (cl x), (fun m' m => (get_post (cl x)) m' m /\ proc_call x m m' ps)).
+  fun x => (get_pre (cl x),
+          (fun m' m => (get_post (cl x)) m' m /\ proc_call x m m' ps)).
 
 (* Facts about phi_call *)
 
 Lemma phi_call_hoare (ps: Psi.psi) (cl : Phi.phi) :
   (forall p, hoare_triple (get_pre (cl p)) (get_post (cl p)) (CCall p) ps) ->
-  (forall p, hoare_triple (get_pre (phi_call cl ps p)) (get_post (phi_call cl ps p)) (CCall p) ps).
+  (forall p, hoare_triple
+          (get_pre (phi_call cl ps p))
+          (get_post (phi_call cl ps p))
+          (CCall p) ps).
 Proof.
 intros.
 intros s s' Hpre Heval.
@@ -424,130 +174,52 @@ Qed.
 
 Lemma rela_hoare_extract rcl ps:
   (forall p : list Proc.Proc.t,
-    0 < length p -> relational_prop (get_r_pre (rcl p)) (get_r_post (rcl p)) (fold_call p) ps) ->
-   (forall p, hoare_triple (get_pre ((extract rcl) p)) (get_post ((extract rcl) p)) (CCall p) ps).
+      0 < length p ->
+      relational_prop
+        (get_r_pre (rcl p))
+        (get_r_post (rcl p))
+        (fold_call p) ps) ->
+  (forall p, hoare_triple
+          (get_pre ((extract rcl) p))
+          (get_post ((extract rcl) p)) (CCall p) ps).
 Proof.
-intros.
-assert (H1 : 0 < 1); auto.
-specialize (H [p] H1). simpl in H.
-apply Single_Rela_Prop.one_rela_is_hoare.
-simpl.
-intros s s' hy1 hy2 Hpre Heval.
-inversion hy1.
-inversion hy2.
-rewrite hd_length_1 by apply H3.
-rewrite hd_length_1 by apply H2.
-apply H. all: try assumption.
-rewrite hd_length_1 in Hpre by apply H2.
-assumption.
+  intros.
+  assert (H1 : 0 < 1); auto.
+  specialize (H [p] H1). simpl in H.
+  apply Single_Rela_Prop.one_rela_is_hoare.
+  simpl.
+  intros s s' hy1 hy2 Hpre Heval.
+  inversion hy1.
+  inversion hy2.
+  rewrite hd_length_1 by apply H3.
+  rewrite hd_length_1 by apply H2.
+  apply H. all: try assumption.
+  rewrite hd_length_1 in Hpre by apply H2.
+  assumption.
 Qed.
 
 (** Definition of a relational verification condition generator for procedures **)
 
 Definition rtc_p (ps: Psi.psi) (rcl : R_Phi.phi) : Prop :=
     forall f m ps',
-    let c := (map ps f) in
+    let c := fold_proc ps f in
     let h := (map (fun _ => empty_history) f) in
-    forall (hy1:length c = length m) (hy2:length c = length h),
+    let cl := phi_call (extract rcl) ps' in
     (get_r_pre (rcl f)) m -> tr rcl ps' ->
-              rtc' c m h (phi_call (extract rcl) ps') hy1 hy2 /\
-              rtc c m h (phi_call (extract rcl) ps')
-                                       (fun m' _ => (get_r_post (rcl f)) m' m) hy1 hy2.
+    rtc' c m h cl /\  rtc c m h cl (fun m' _ => (get_r_post (rcl f)) m' m).
 
-(* Facts about relational verification condition generator for procedures *)
-
-Lemma simpl_rtc' :
-  forall (a:Proc.Proc.t) f (s:sigma) m ps ps' phi
-   (hy1:length (map ps (a::f)) = length (s::m))
-   (hy2:length (map ps (a::f)) =
-        length (map (fun _ : Proc.Proc.t => empty_history) (a :: f))),
-  exists H1, exists H2,
-       rtc' (map ps (a :: f))
-            (s :: m)
-            (map (fun _ : Proc.Proc.t => empty_history) (a :: f))
-            (phi_call (extract phi) ps') hy1 hy2 =
-       rtc' (ps a :: map ps f)
-            (s :: m)
-            (empty_history :: map (fun _ : Proc.Proc.t => empty_history) f)
-            (phi_call (extract phi) ps') H1 H2.
+Lemma get_r_pre_emphi_false m f :
+  get_r_pre (R_Phi.empty_phi f) m -> False.
 Proof.
- eexists. eexists. program_simpl.
-Qed.
-
-Lemma simpl_rtc :
-  forall (a:Proc.Proc.t) f (s:sigma) m ps
-   (hy1:length (map Psi.empty_psi (a::f)) = length (s::m))
-   (hy2:length (map Psi.empty_psi (a::f)) =
-        length (map (fun _ : Proc.Proc.t => empty_history) (a :: f))),
-  exists H1, exists H2,
-  forall suite,
-       rtc (map Psi.empty_psi (a :: f))
-            (s :: m)
-            (map (fun _ : Proc.Proc.t => empty_history) (a :: f))
-            (phi_call (extract R_Phi.empty_phi) ps)
-            suite hy1 hy2 =
-       rtc (CSkip :: map Psi.empty_psi f)
-            (s :: m)
-            (empty_history :: map (fun _ : Proc.Proc.t => empty_history) f)
-            (phi_call (extract R_Phi.empty_phi) ps)
-            suite H1 H2.
-Proof.
-  eexists. eexists. intros. program_simpl.
+  simpl.
+  unfold empty_r_precondition.
+  auto.
 Qed.
 
 Lemma rtc_p_empty_psi : rtc_p Psi.empty_psi R_Phi.empty_phi.
 Proof.
-unfold rtc_p.
-intros.
-split.
-* generalize dependent m.
-  induction f;intros.
-  + inversion hy1.
-    symmetry in H2.
-    apply length_zero_iff_nil in H2.
-    subst.
-    simpl.
-    auto.
-  + destruct m;[ discriminate hy1 | ].
-    destruct (simpl_rtc' a f s m
-                         Psi.empty_psi ps' R_Phi.empty_phi hy1 hy2)
-       as (hyr1 & hyr2 & HYP).
-    rewrite HYP.
-    clear HYP.
-    destruct (mk_rtc'_def _ _ (phi_call (extract R_Phi.empty_phi) ps')
-                          _ _  _ _ hyr1 hyr2)
-          as (hyr3 & hyr4 & HYP).
-    rewrite HYP.
-    clear HYP.
-    split.
-    - simpl.
-      auto.
-    - apply IHf.
-      simpl.
-      unfold empty_r_precondition.
-      auto.
-* generalize dependent m.
-  induction f; intros.
-  + inversion hy1.
-    symmetry in H2.
-    apply length_zero_iff_nil in H2.
-    subst.
-    simpl.
-    unfold empty_r_postcondition.
-    auto.
-  + destruct m; [discriminate hy1 | ].
-    destruct (simpl_rtc a f s m ps' hy1 hy2) as (hyr1 & hyr2 & HYP).
-    rewrite HYP.
-    clear HYP.
-    destruct (mk_rtc_def _ _ (phi_call (extract R_Phi.empty_phi) ps')
-                          _ _ _ _ hyr1 hyr2)
-             as (hyr3 & hyr4 & HYP).
-    rewrite HYP.
-    clear HYP.
-    simpl.
-    intros.
-    apply IHf.
-    simpl.
-    unfold empty_r_precondition.
-    auto.
+  unfold rtc_p.
+  intros.
+  apply get_r_pre_emphi_false in H.
+  contradiction H.
 Qed.
