Correct_Rela.v
@@ -5,121 +5,87 @@ From Rela Require Import Correct.
 From Rela Require Import Rela.
 From Rela Require Import Vcg.
 From Rela Require Import Vcg_Rela.
-From Rela Require Import Quadruple.
-From Rela Require Import Vcg_Quadruple.
 
-From Coq Require Import Program.
-From Coq Require Import Eqdep_dec.
-From Coq Require Import Lists.List.
+From Stdlib Require Import Lists.List.
 Import ListNotations.
-From Coq Require Import Lia.
 
 (** Proof that one can use a standard verification condition generator
     to proof Relational Properties **)
 
 Lemma rcorrect_c :
-forall rcl ps p h (hyh :length p = length h),
+forall rcl ps p h,
 forall (P: r_precondition) (Q: r_postcondition),
-(forall ps,
-  (forall ml (hy:length p = length ml),
-      P ml -> tr rcl ps ->
-      rtc' p ml h (phi_call (extract rcl) ps) hy hyh)
-  /\
-  (forall ml (hy:length p = length ml),
-     P ml -> tr rcl ps ->
-     rtc p ml h (phi_call (extract rcl) ps ) (fun ml' _ => Q ml' ml) hy hyh)) ->
-relational_prop_ctx rcl ps P Q p.
+  (forall ps,
+      let cll := (phi_call (extract rcl)) ps in
+      (forall ml,  P ml -> tr rcl ps ->  rtc' p ml h cll)  /\
+      (forall ml, P ml -> tr rcl ps -> rtc p ml h cll (fun ml' _ => Q ml' ml)))
+  ->
+  relational_prop_ctx rcl ps P Q p.
 Proof.
-intros rcl ps p h hyh P Q H.
-specialize (H ps); destruct H.
-generalize dependent H0.
-generalize dependent H.
-generalize dependent Q.
-generalize dependent P.
-generalize dependent h.
-induction p;intros.
-*  intros Hproc.
-   unfold relational_prop.
-   intros.
-   specialize (H0 []).
-   inversion hyh.
-   symmetry in H6.
-   apply length_zero_iff_nil in H6.
-   subst.
-   simpl in H0.
-   apply length_zero_iff_nil in H1.
-   apply length_zero_iff_nil in H2.
-   subst.
-   eapply H0.
-   reflexivity.
-   assumption.
-   eapply tr_relational_prop.
-   apply Hproc.
-*  intros Hproc.
-   unfold relational_prop.
-   intros.
-   destruct s;[ discriminate H1 | ].
-   destruct s';[ discriminate H2 | ].
-   destruct h;[ discriminate hyh | ].
-   inversion H4;subst.
-   inversion hyh.
-   specialize (IHp (h0) H6 (fun sl => P (s :: sl))
-                           (fun sl' sl => Q (s1 :: sl') (s :: sl))).
-   simpl in IHp.
-   generalize H13.
-   generalize H3.
-   inversion H1.
-   inversion H2.
-   generalize H8.
-   generalize H7.
-   eapply IHp.
-    ** intros.
-       assert (hy2: length (a ::p) = length (s::ml)).
-       {intros. simpl. rewrite hy. reflexivity. }
-       specialize (H (s :: ml) hy2 H5).
-       destruct (mk_rtc'_def a p (phi_call (extract rcl) ps) s ml h h0 hy2 hyh)
-          as (hyr1 & hyr2 & HYP).
-       rewrite HYP in H.
-       destruct H.
-       apply tr_relational_prop.
-       apply Hproc.
-       replace hy with hyr1.
-       replace H6 with hyr2.
-       apply H11.
-       apply eq_proofs_unicity. intros. lia.
-       apply eq_proofs_unicity. intros. lia.
-    ** intros.
-       generalize H10.
-       generalize H5.
-       generalize s s1.
-       rewrite hoare_rela.
-       specialize (rela_hoare_extract rcl ps Hproc).
-       apply tr_relational_prop in Hproc.
-       intros.
-       specialize (phi_call_hoare ps (fun p => extract rcl p) H11) .
-       eapply correct_c.
-       -- intros.
-          assert (hy2: length (a ::p) = length (m::ml)).
-          {intros. simpl. rewrite hy. reflexivity. }
-          specialize (H (m :: ml) hy2 H12 Hproc).
-          destruct (mk_rtc'_def a p (phi_call (extract rcl)ps) m ml h h0 hy2 hyh)
-            as (hyr1 & hyr2 & HYP).
-          rewrite HYP in H.
-          apply H.
-       -- intros.
-          assert (hy2: length (a ::p) = length (m::ml)).
-          {intros. simpl. rewrite hy. reflexivity. }
-          destruct (mk_rtc_def a p (phi_call (extract rcl) ps) m ml h h0 hy2 hyh)
-             as (hyr1 & hyr2 & HYP).
-          specialize (H0 (m::ml) hy2 H12 Hproc).
-          specialize (HYP (fun l _ => Q l (m ::ml))).
-          rewrite HYP in H0.
-          replace hy with hyr1.
-          replace H6 with hyr2.
-          apply H0.
-          apply eq_proofs_unicity.  intros. lia.
-          apply eq_proofs_unicity.  intros. lia.
-     ** apply Hproc.
+  intros rcl ps p h P Q H.
+  specialize (H ps); destruct H.
+  generalize dependent H0.
+  generalize dependent H.
+  generalize dependent Q.
+  generalize dependent P.
+  generalize dependent h.
+  induction p;intros.
+  -  intros Hproc.
+     unfold relational_prop.
+     intros.
+     apply length_zero_iff_nil in H1.
+     apply length_zero_iff_nil in H2.
+     subst.
+     destruct h.
+     + apply (H0 []).
+        * assumption.
+        * apply tr_relational_prop.
+          apply Hproc.
+     + assert (Htr: tr rcl ps).
+       { apply tr_relational_prop. apply Hproc. }
+       specialize (H0 [] H3 Htr).
+       contradiction H0.
+  -  intros Hproc.
+     unfold relational_prop.
+     intros.
+     destruct s;[ discriminate H1 | ].
+     destruct s';[ discriminate H2 | ].
+     inversion H4;subst.
+     destruct h.
+     + assert (Htr: tr rcl ps).
+       { apply tr_relational_prop.  apply Hproc. }
+       specialize (H0 (s :: s0) H3 Htr).
+       contradiction H0.
+     + specialize (IHp h0 (fun sl => P (s :: sl))
+                     (fun sl' sl => Q (s1 :: sl') (s :: sl))).
+       simpl in IHp.
+       generalize H13.
+       generalize H3.
+       inversion H1.
+       inversion H2.
+       generalize H7.
+       generalize H6.
+       apply IHp.
+       * intros.
+         specialize (H (s :: ml) H5 H8).
+         apply H.
+       * intros.
+         generalize H10.
+         generalize H5.
+         generalize s s1.
+         rewrite hoare_rela.
+         specialize (rela_hoare_extract rcl ps Hproc).
+         apply tr_relational_prop in Hproc.
+         intros.
+         specialize (phi_call_hoare ps (fun p => extract rcl p) H9) .
+         eapply correct_c.
+         -- intros.
+            specialize (H (m :: ml) H11 Hproc).
+            apply H.
+         -- intros.
+            specialize (H0 (m::ml) H11 Hproc).
+            apply H0.
+       * apply Hproc.
 Qed.
 
 (** Proof that one can use a verification condition
@@ -130,96 +96,36 @@ Lemma rcorrect_proc :
     rtc_p ps rcl ->
     relational_prop_proc_ctx rcl ps.
 Proof.
-  intros cl ps Htc.
+  intros rcl ps Htc.
   unfold relational_prop_proc_ctx.
   intros.
-  assert (H1:length (map ps p) = length (map (fun _ => empty_history) p)).
-  {  rewrite map_length. rewrite map_length. reflexivity. }
   unfold rtc_p in Htc.
-  eapply rcorrect_c;split;intros; specialize (Htc p ml ps1 hy H1 H);destruct Htc.
+  eapply rcorrect_c;split;intros; specialize (Htc p ml ps1);destruct Htc.
   * assumption.
-  * apply H2.
   * assumption.
-  * apply H3.
+  * apply H1.
+  * assumption.
+  * assumption.
+  * assumption.
 Qed.
 
 (** Proof that one can use a verification condition
     generator for modular Relatioanl Properties verification **)
 
 Theorem rcorrect :
-  forall rcl ps p h (hyh :length p = length h),
+  forall rcl ps p h,
   forall (P: r_precondition) (Q: r_postcondition),
   rtc_p ps rcl ->
   (forall ps,
-    (forall ml (hy:length p = length ml),
-       P ml -> tr rcl ps -> rtc' p ml h (phi_call (extract rcl) ps) hy hyh) /\
-    (forall ml (hy:length p = length ml),
+    (forall ml,
+       P ml -> tr rcl ps -> rtc' p ml h (phi_call (extract rcl) ps)) /\
+    (forall ml,
        P ml -> tr rcl ps ->
-       rtc p ml h (phi_call (extract rcl) ps ) (fun ml' _ => Q ml' ml) hy hyh)) ->
+       rtc p ml h (phi_call (extract rcl) ps ) (fun ml' _ => Q ml' ml))) ->
     relational_prop P Q p ps.
 Proof.
-intros.
-apply recursion_relational with rcl.
-* apply rcorrect_proc. assumption.
-* apply rcorrect_c with (h:=h) (hyh:=hyh). all: try assumption.
+  intros.
+  apply recursion_relational with rcl.
+  * apply rcorrect_proc. assumption.
+  * apply rcorrect_c with (h:=h). all: try assumption.
 Qed.
-
-(** Extention: We add quadruple with speciale rules **)
-
-(** Proof that one can use a verification condition
-    generator to proof Quadruple on procedure **)
-
-Lemma qcorrect_proc :
-  forall qcl cl ps,
-    qtc_p ps cl qcl ->
-    quadruple_proc_ctx qcl ps.
-Proof.
-Admitted.
-
-(** Proof that one can use a verification condition
-    generator for modular Relatioanl Properties verification
-    (with handler of Quadruples)
- **)
-
-(* Add to the one sided rule a termination requireement to get RHL
-
-WE WANT RHL
-
- *)
-
-
-(*
-
-- We need to define how to verifiy quadruples using verification
-  condition generation using proof on calls and loops.
-- We need to define how proof relational properties using
-  relational properties on calls, quadruples on calls and
-  quadruple on whiles
-
- *)
-
-(* Include the relational while rule system *)
-
-(* Just use the normal termination for the transitivity application, for
- partial correction use axiom forall f, s, exit s', call f s s'
- and proof the rule from the phd *)
-
-Theorem qrcorrect :
-  forall rcl (qcl: Quadruple.Q_Phi.phi) ps p h (hyh :length p = length h),
-  forall (P: r_precondition) (Q: r_postcondition),
-  rtc_p ps rcl ->
-  qtc_p ps (extract rcl) qcl ->
-  (forall ps,
-    (forall ml (hy:length p = length ml),
-       P ml -> tr rcl ps -> rtc' p ml h (phi_call (extract rcl) ps) hy hyh) /\
-    (forall ml (hy:length p = length ml),
-       P ml -> tr rcl ps ->
-       rtc p ml h (phi_call (extract rcl) ps ) (fun ml' _ => Q ml' ml) hy hyh)) ->
-    relational_prop P Q p ps.
-Proof.
-intros.
-apply ext_recursion_relational with rcl qcl.
-* eapply qcorrect_proc. apply H0.
-* apply rcorrect_proc. assumption.
-* apply rcorrect_c with (h:=h) (hyh:=hyh). all: try assumption.
-  Admitted.
